lean/Och.lean
@@ -1,7 +1,5 @@
 import Och.Syntax
 import Och.Eval
 import Och.Subtyping
-import Och.ValSub
 import Och.Soundness
-import Och.Monotonicity
 import Och.Tests
